Another restructure heavily inspired by a certain XSalsa formalisation. Also almost finished one half of the middle proof.

theories/algebra/NR_PRF.ec
@@ -1,6 +1,6 @@
 (* NR-PRF *)
 require import Int Real List SmtMap Distr DList FSet.
-require (*--*) GroupAction.
+require (*--*) GroupAction PRF.
 
 (* We need a regular, effective, abelian group action for this construction *) 
 clone import GroupAction.ARegEGA as Ega.
@@ -10,96 +10,72 @@ type K = group * group.
 type D = bool. (* Only one bit for the moment but will be an l-bit word *) 
 type R = set.
 
-(* This is the construction we wish to prove is a PRF *)
+(* This is the Naor-style PRF construction *)
 op F (k : K) (m : D) =
     if   m
     then act (k.`1 * k.`2) x0
     else act k.`1 x0.
 
 (* Setup the uniform distribution on our range *)
-clone import MFinite as DR with
-    type t <- R.
-op dR = DR.dunifin.
-lemma dR_ll (x : D) : is_lossless dR.
-proof.
-exact DR.dunifin_ll.
-qed. 
+clone import MFinite as Uni_dR with
+    type t <- R
+rename
+    "dunifin" as "dR".
 
-op dK : K distr = sample `*` sample.
-lemma dK_ll : is_lossless dK.
-proof.
+(* Setting up the PRF *)
+clone import PRF as PRF_t with
+    type D <- D,
+    type R <- R.
+
+clone import RF as NS_RF with
+    op dR _ <- dR
+proof *.
+realize dR_ll.
+by move=> _; exact dR_ll.
+qed.
+
+clone import PseudoRF as NS_PRF with
+    type K <- K,
+    op dK <- sample `*` sample,
+    op F <- F
+proof *.
+realize dK_ll.
 apply dprod_ll.
 split; exact DG.dunifin_ll.
 qed.
 
 (* ------------------------------------------------------ *)
-(* Setup the bounded PRF games/oracles/adversaries *)
+(* Setup our bounding module *)
 
 module type Bounded_PRF = {
-    proc init(Q : int) : unit
+    proc init(_ : int) : unit
     proc f(_ : D) : R
 }.
 
-module type PRF_Oracles = {
-    proc f(_ : D) : R
-}.
-
-module type Distinguisher (F : PRF_Oracles) = {
-    proc distinguish() : bool
-}.
-
-module Bounded_PRF_IND (F : Bounded_PRF) (D : Distinguisher) = {
-    proc main(Q : int) : bool = {
-        var b;
+module Bounded_PRF_IND (F : Bounded_PRF) (A : Distinguisher) = {
+    proc main (Q : int) : bool = {
+        var b : bool;
         F.init(Q);
-        b <@ D(F).distinguish();
+        b <@ A(F).distinguish();
         return b;
     }
 }.
 
-module Bounded_PRF_Real = {
-    var k : K
+module BoundPRF(O : PRF_t.PRF) : Bounded_PRF = {
     var c, q : int
     
     proc init(Q : int) : unit = {
-        k <$ dK;
+        O.init();
         q <- Q;
         c <- 1;
     }
 
     proc f(x : D) : R = {
         var val : R;
+        val <- witness;
         if (c <= q) {
-            val <- F k x;
+            val <@ O.f(x);
             c <- c + 1;
-        } else {
-            val <- witness;
-        }        
-        return val;
-    }
-}.
-
-module Bounded_PRF_Ideal = {
-    var c, q : int
-    var m : (D, R) fmap
-
-    proc init(Q : int): unit = {
-        q <- Q;
-        c <- 1;
-        m <- empty;
-    }
-
-    proc f(x : D) : R = {
-        var val : R;
-        if (c <= q) {
-            if (x \notin m) {
-                val <$ dR;
-                m.[x] <- val;
-            }
-            val <- (oget m.[x]);
-            c <- c + 1;
-        } else {
-            val <- witness;
         }
         return val;
     }
@@ -109,51 +85,48 @@ module Bounded_PRF_Ideal = {
 (* Lemma 4.21 *)
 (* Start by just considering the case when l = 1, here we will just have two games for an adversary to distinguish *)
 
-module type Hybrid_PRF = {
-    proc init(_ : int) : unit
-    proc doit(_ : D) : R
-}.
-
-module type WPR_Oracles = {
-    proc doit(_ : D) : R
-}.
-
-module type Hybrid_PRF_Adv (O : WPR_Oracles) = {
-    proc distinguish() : bool
-}.
-
-module Hybrid_PRF_IND (H : Hybrid_PRF) (A : Hybrid_PRF_Adv) = {
-    proc main (Q : int) : bool = {
-        var b : bool;
-        H.init(Q);
-        b <@ A(H).distinguish();
-        return b;
-    }
-}.
-
 module Hybrid_PRF_0 = {
     var g0, g1 : group
-    var c, q : int
 
-    proc init(Q : int) = {
+    proc init() = {
         g0 <$ sample;
         g1 <$ sample;
-        q <- Q;
-        c <- 1;
     }
 
-    proc doit(s) = {
+    proc f(s) = {
         var val;
+        val <- act g0 x0;
+        if (s) {
+            val <- act g1 val;
+        }
+        return val;
+    }
+}.
 
-        (* Make sure we can't make more than Q, 'proper', queries *)
-        if (c <= q) {
-            val <- act g0 x0;
-            if (s) {
-                val <- act g1 val;
-            }
-            c <- c + 1;
-        } else {
-            val <- witness;
+module Hybrid_PRF_0' = {
+    var m : (int, group) fmap
+    var g1 : group
+
+    proc init() = {
+        g1 <$ sample;
+        m <- empty;
+    }
+
+    proc get(i : int) : group = {
+        var g;
+        if (i \notin m) {
+            g <$ sample;
+            m.[i] <- g;    
+        }
+        return oget m.[i];
+    }
+
+    proc f(s) = {
+        var val, g;
+        g <@ get(0);
+        val <- act g x0;
+        if (s) {
+            val <- act g1 val;
         }
         return val;
     }
@@ -161,224 +134,116 @@ module Hybrid_PRF_0 = {
 
 module Hybrid_PRF_L = {
     var m : (D, R) fmap
-    var q, c : int
-  
-    proc init(Q : int) = {
-        q <- Q;
-        c <- 1;
+
+    proc init() = {
         m <- empty;
     }
 
-    proc doit(s) = {
-        var gq, val;
-        if (c <= q) {
-            if (s \notin m) {
-                gq <$ sample;
-                val <- act gq x0;
-                m.[s] <- val;
-            } else {
-                val <- oget m.[s];
-            }
-            c <- c + 1;
-        } else {
-            val <- witness;
+    proc f(s) = {
+        var gq;
+        if (s \notin m) {
+            gq <$ sample;
+            m.[s] <- act gq x0;
         }
-        return val;
-    }
-}.
-
-(* Simply wrap around the distinguisher for a PRF *)
-module (A (D : Distinguisher) : Hybrid_PRF_Adv) (F : WPR_Oracles) = {
-    module O = {
-        proc f = F.doit
-    }
-
-    proc distinguish() = {
-        var b;
-
-        b <@ D(O).distinguish();
-        return b;
+        return oget m.[s];
     }
 }.
 
 (** |Pr[IND(PRF, D).main() @ &m: res] - Pr[IND(RF, D).main() @ &m: res]|
     <= Advantage of A(D) against something we think is hard **)
 
+lemma sample_dR_iso g x: mu1 sample g = mu1 dR (act g x).
+proof.
+have /= <- := dmap1E_can dR (extract x) (fun g=> act g x) g _ _.
++ by rewrite /cancel=> g'; rewrite -extractUniq.
++ by move=> a _ /=; rewrite extractP.
+congr; apply: eq_funi_ll.
++ exact: DG.dunifin_funi.
++ exact: DG.dunifin_ll.
++ apply/dmap_funi.
+  + exists (fun g=> act g x); split.
+    + by move=> a; exact: extractP.
+    by move=> h; rewrite -extractUniq.
+  exact: dR_funi.
+exact/dmap_ll/Uni_dR.dR_ll.
+qed.
+
 require (*--*) DProd.
 clone DProd.ProdSampling with
   type t1 <- group,
   type t2 <- group.
 
-lemma Hybrid_PRF_0_PRF_Real_eq (D <: Distinguisher {Hybrid_PRF_0, Bounded_PRF_Real}) (x : int) &m:
-  Pr[Bounded_PRF_IND(Bounded_PRF_Real, D).main(x) @ &m: res] = Pr[Hybrid_PRF_IND(Hybrid_PRF_0, A(D)).main(x) @ &m: res].
+lemma Hybrid_PRF_0_PRF_eq (D <: Distinguisher {Hybrid_PRF_0, BoundPRF, PRF}) (x : int) &m:
+  Pr[Bounded_PRF_IND(BoundPRF(PRF), D).main(x) @ &m: res] = Pr[Bounded_PRF_IND(BoundPRF(Hybrid_PRF_0), D).main(x) @ &m: res].
 proof.
 byequiv=> //.
 proc.
 inline *.
 sp.
-seq  1  2: (={glob D, Q, Q0}
-            /\ Bounded_PRF_Real.k{1} = (Hybrid_PRF_0.g0,Hybrid_PRF_0.g1){2}
-            ).
+seq 1 2: (   ={glob D, Q, Q0}
+          /\ NS_PRF.PRF.k{1} = (Hybrid_PRF_0.g0,Hybrid_PRF_0.g1){2}).
 + conseq />.
   transitivity {1} (** Which memory should the piece of code operate in? **)
-               { Bounded_PRF_Real.k <@ ProdSampling.S.sample(sample, sample); } (** Which piece of code? **)
-               (true ==> ={Bounded_PRF_Real.k}) (** Left-to-step similarity **)
-               (true ==> Bounded_PRF_Real.k{1} = (Hybrid_PRF_0.g0, Hybrid_PRF_0.g1){2}) (** Step-to-right similarity **)=> //.
+               {PRF.k <@ ProdSampling.S.sample(sample, sample); } (** Which piece of code? **)
+               (true ==> ={PRF.k}) (** Left-to-step similarity **)
+               (true ==> PRF.k{1} = (Hybrid_PRF_0.g0, Hybrid_PRF_0.g1){2}) (** Step-to-right similarity **)=> //.
   + by inline {2} 1; auto.
   transitivity {2}
                { (Hybrid_PRF_0.g0, Hybrid_PRF_0.g1) <@ ProdSampling.S.sample2(sample, sample); }
-               ( true ==> Bounded_PRF_Real.k{1} = (Hybrid_PRF_0.g0, Hybrid_PRF_0.g1){2})
+               (true ==> PRF.k{1} = (Hybrid_PRF_0.g0, Hybrid_PRF_0.g1){2})
                (true ==> ={Hybrid_PRF_0.g0, Hybrid_PRF_0.g1})=> //.
   + by call ProdSampling.sample_sample2; auto=> /> [].
   by inline {1} 1; auto.
 wp.
 sp.
-call (: Bounded_PRF_Real.k{1} = (Hybrid_PRF_0.g0, Hybrid_PRF_0.g1){2}
-      /\ Bounded_PRF_Real.c{1} = Hybrid_PRF_0.c{2}
-      /\ Bounded_PRF_Real.q{1} = Hybrid_PRF_0.q{2}
-      ).
-+ proc; wp; skip=> />.
+call (:  PRF.k{1} = (Hybrid_PRF_0.g0, Hybrid_PRF_0.g1){2}
+      /\ ={BoundPRF.c, BoundPRF.q}).
++ proc; inline*; wp; skip=> />.
   move=> &2 _ _ @/F /=.  
   rewrite comp.
   exact: actC.
 skip=> />.
 qed.
 
-lemma Hybrid_PRF_L_PRF_Real_eq (D <: Distinguisher {Hybrid_PRF_L, Bounded_PRF_Ideal}) (a : int) &m:
-    Pr[Bounded_PRF_IND(Bounded_PRF_Ideal, D).main(a) @ &m: res] = Pr[Hybrid_PRF_IND(Hybrid_PRF_L, A(D)).main(a) @ &m: res].
+lemma Hybrid_PRF_L_RF_eq (D <: Distinguisher {Hybrid_PRF_L, RF, BoundPRF}) (a : int) &m:
+    Pr[Bounded_PRF_IND(BoundPRF(RF), D).main(a) @ &m: res] = Pr[Bounded_PRF_IND(BoundPRF(Hybrid_PRF_L), D).main(a) @ &m: res].
 proof.
 byequiv (_ : ={glob D, arg} ==> ={res})=> //.
 proc.
 inline *.
 wp.
-sp.
-call (:  Bounded_PRF_Ideal.m{1} = Hybrid_PRF_L.m{2}
-      /\ Bounded_PRF_Ideal.c{1} = Hybrid_PRF_L.c{2}
-      /\ Bounded_PRF_Ideal.q{1} = Hybrid_PRF_L.q{2}
-      ).
-+ proc.
-  if.
-  + by move=> />.
-  + if.
+call (: ={m}(RF, Hybrid_PRF_L) /\ ={BoundPRF.c, BoundPRF.q}).
++ proc; inline*.
+  sp.
+  if; first by move=> />.
+  + sp.
+    if.
     + by move=> />.
-    + seq 1 2 : (x{1} = s{2}
-                /\ ={val}
-                /\ Bounded_PRF_Ideal.m{1} = Hybrid_PRF_L.m{2}
-                /\ Bounded_PRF_Ideal.c{1} = Hybrid_PRF_L.c{2}
-                /\ Bounded_PRF_Ideal.q{1} = Hybrid_PRF_L.q{2}
-                ).
-      + wp.
-        rnd (fun x => extract x0 x) (fun g => act g x0).
-        skip=> &1 &2.
-        do case => eq1 eq2 _ _ />.
-        split.
-        + move=> g _.
-          exact extractUniq.
-        move=> _.
-        split.
-        + move=> g _.
-          have /= <- := dmap1E_can DR.dunifin (extract x0) (fun g=> act g x0) g _ _.
-            + by rewrite /cancel=> g'; rewrite -extractUniq.
-            + by move=> x _ /=; rewrite extractP.
-          congr; apply: eq_funi_ll.
-          + exact: DG.dunifin_funi.
-          + exact: DG.dunifin_ll.
-          + apply/dmap_funi.
-            + exists (fun g=> act g x0); split.
-              + by move=> x; exact: extractP.
-              by move=> h; rewrite -extractUniq.
-            exact: dunifin_funi.
-          exact/dmap_ll/dunifin_ll.
-        move=> _ r rin.
-        by rewrite extractP.
-      wp.
-      skip.
-      move=> &1 &2 />.
-      rewrite get_set_sameE.
-      trivial.
-    wp.
-    by skip.
-  wp.
-  by skip.
-by skip.
+    + wp.
+      rnd (fun x => extract x0 x) (fun g => act g x0).
+      skip=> &1 &2 /> _ _.
+      split=> [g _ | _]; first exact extractUniq.
+      split=> [g _ | _ r _]; first exact sample_dR_iso.
+      by rewrite extractP.
+    auto=> &1 &2 />.
+  by auto.
+by auto.
+qed.
+
+lemma PRF_Hybrid_PRF_Reduction (D <: Distinguisher {BoundPRF, Hybrid_PRF_0, Hybrid_PRF_L, PRF, RF}) (x : int) &m :
+  `|Pr[Bounded_PRF_IND(BoundPRF(PRF), D).main(x) @ &m: res] - Pr[Bounded_PRF_IND(BoundPRF(RF), D).main(x) @ &m: res]|
+= `|Pr[Bounded_PRF_IND(BoundPRF(Hybrid_PRF_0), D).main(x) @ &m: res] - Pr[Bounded_PRF_IND(BoundPRF(Hybrid_PRF_L), D).main(x) @ &m: res]|.
+by rewrite (Hybrid_PRF_0_PRF_eq D) (Hybrid_PRF_L_RF_eq D).
 qed.
 
 (* ----------------------------------------------- *)
-module type Hybrid_WPR = {
-    proc init(_ : int) : unit
-    proc query() : R * R
-}.
-
-module type H_WPR_Oracles = {
-    proc query() : R * R
-}.
-
-module type Hybrid_WPR_Adv (F : H_WPR_Oracles) = {
-    proc solve() : bool
-}.
-
-module Hybrid_WPR_IND (H : Hybrid_WPR) (A : Hybrid_WPR_Adv) = {
-    proc main(Q : int) : bool = {
-        var b : bool;
-        H.init(Q);
-        b <@ A(H).solve();
-        return b;
-    }
-}.
-
-module Hybrid_WPR_Real = {
-    var q, c : int
-    var gt : group
-  
-    proc init(Q : int) = {
-        gt <$ sample;
-        q <- Q;
-        c <- 1;
-    }
-
-    proc query() = {
-        var gq, xq, yq;
-        var xy;
-        if (c <= q) {
-            gq <$ sample;
-            xq <- act gq x0;
-            yq <- act gt xq;
-            xy <- (xq, yq);
-            c <- c + 1;
-        } else {
-            xy <- witness;
-        }
-        return xy;
-    }
-}.
-
-module Hybrid_WPR_Ideal = {
-    var q, c : int
-  
-    proc init(Q : int) = {
-        q <- Q;
-        c <- 1;
-    }
-    
-    proc query() = {
-        var gq, hq, xq, yq;
-        var xy;
-        if (c <= q) {
-            gq <$ sample;
-            xq <- act gq x0;
-            hq <$ sample;
-            yq <- act hq xq;
-            xy <- (xq, yq);
-            c <- c + 1;
-        } else {
-            xy <- witness;
-        }
-        return xy;
-    }
-}.
-
 (* Weak pseudorandomness assumption *)
 module type WP = {
+    proc init() : unit
+    proc query() : R * R
+}.
+
+module type Bounded_WP = {
     proc init(_ : int) : unit
     proc query() : R * R
 }.
@@ -392,178 +257,215 @@ module type WP_Adv (F : WP_Oracles) = {
 }.
 
 module WP_IND (F : WP) (A : WP_Adv) = {
-  proc main (Q : int) : bool = {
+  proc main() : bool = {
     var b : bool;
-    F.init(Q);
+    F.init();
     b <@ A(F).distinguish();
     return b;
   }
 }.
 
-module WP_Real = {
+module BoundWP(O : WP) : Bounded_WP = {
     var q, c : int
-    var g : group
-  
     proc init(Q : int) = {
-        g <$ sample;
+        O.init();
         q <- Q;
         c <- 1;
     }
 
     proc query() = {
         var r : set * set;
-        var xq, yq : set;
+        r <- witness;
         if (c <= q) {
-            xq <$ dR;
-            yq <- act g xq;
-            r <- (xq, yq);
-            c <- c + 1;
-        } else {
-            r <- witness;
+            r <@ O.query();
         }
         return r;
+    }
+}.
+
+module WP_Real = {
+    var g : group
+  
+    proc init() = { g <$ sample; }
+
+    proc query() = {
+        var xq, yq : set;
+        xq <$ dR;
+        yq <- act g xq;
+        return (xq, yq);
     }
 }.
 
 module WP_Ideal = {
-    var q, c : int
-
-    proc init(Q : int) = {
-        q <- Q;
-        c <- 1;
-    }
+    proc init() = { }
 
     proc query() = {
-        var r : set * set;
         var xq, yq : set;
-        if (c <= q) {
-            xq <$ dR;
-            yq <$ dR;
-            r <- (xq, yq);
-            c <- c + 1;
-        } else {
-            r <- witness;
-        }
-        return r;
+        xq <$ dR;
+        yq <$ dR;
+        return (xq, yq);
     }
 }.
 
-(* Reduction from Hybrid_WPR to WP *)
-module (B1 (A : Hybrid_WPR_Adv) : WP_Adv) (F : WP_Oracles) = {
+module Hybrid_WP_Real = {
+    var gt : group
+
+    proc init() = { gt <$ sample; }
+
+    proc query() = {
+        var gq, xq, yq;
+        gq <$ sample;
+        xq <- act gq x0;
+        yq <- act gt xq;
+        return (xq, yq);
+    }
+}.
+
+module Hybrid_WP_Ideal = {
+    proc init() = { }
+
+    proc query() = {
+        var gq, hq, xq, yq;
+        gq <$ sample;
+        xq <- act gq x0;
+        hq <$ sample;
+        yq <- act hq xq;
+        return (xq, yq);
+    }
+}.
+
+lemma Hybrid_WP_WP_Real_eq (A <: WP_Adv{Hybrid_WP_Real, WP_Real}) &m:
+   Pr[WP_IND(WP_Real, A).main() @ &m: res] = Pr[WP_IND(Hybrid_WP_Real, A).main() @ &m: res].
+proof.
+byequiv (: ={glob A, arg} ==> ={res})=> //.
+proc; inline *.
+call (: WP_Real.g{1} = Hybrid_WP_Real.gt{2}).
++ proc; wp.
+  rnd (extract x0) (transpose act x0); auto=> /> &2.
+  split=> [g _ | _]; first exact: extractUniq.
+  split=> [g _ | _ xq _]; first exact: sample_dR_iso.
+  by rewrite extractP.
+by auto=> />.
+qed.
+
+lemma Hybrid_WP_WP_Ideal_eq (A <: WP_Adv{Hybrid_WP_Ideal, WP_Ideal}) &m:
+   Pr[WP_IND(WP_Ideal, A).main() @ &m: res] = Pr[WP_IND(Hybrid_WP_Ideal, A).main() @ &m: res].
+proof.
+byequiv (: ={glob A, arg} ==> ={res})=> //.
+proc.
+inline *.
+call (: true).
++ proc.
+  seq 1 2 : (={xq}).
+  + wp.
+    rnd (fun x => extract x0 x) (fun g => act g x0).
+    skip=> &1 &2 />.
+    split=> [g _ | _]; first exact extractUniq.
+    split=> [g _ | _ r _]; first exact sample_dR_iso.
+    by rewrite extractP.
+  wp.
+  rnd (fun x => extract xq{1} x) (fun g => act g xq{2}).
+  skip=> &1 &2 />.
+  split=> [g _ | _]; first exact extractUniq.
+  split=> [g _ | _ r _]; first exact sample_dR_iso.
+  by rewrite extractP.
+by auto=> />.
+qed.
+
+lemma Hybrid_WP_WP_Reduction (A <: WP_Adv{Hybrid_WP_Ideal, Hybrid_WP_Real, WP_Real, WP_Ideal}) &m :
+`|Pr[WP_IND(Hybrid_WP_Real, A).main() @ &m: res] - Pr[WP_IND(Hybrid_WP_Ideal, A).main() @ &m: res] |
+= `| Pr[WP_IND(WP_Real, A).main() @ &m: res] - Pr[WP_IND(WP_Ideal, A).main() @ &m: res] |.
+by rewrite (Hybrid_WP_WP_Real_eq A) (Hybrid_WP_WP_Ideal_eq A).
+qed.
+
+(* Reduction the middle *)
+
+module (C (D : Distinguisher) : WP_Adv) (F : WP_Oracles) = {
     module O = {
-        proc query = F.query
-    } 
+        var gs : (int, group) fmap
+        var qs : (D, R * R) fmap
+        var j : int
+
+        proc init() = {
+            qs <- empty;
+            j <- 0; (* Hard code the simple variant *)
+        (* More General
+            i <- j + 2;
+            gs <- empty;
+            while (i <= 1) {
+                g <$ sample;
+                gs.[i] <- g;
+                i <- i + 1;
+            }
+        *)
+        }
+
+        proc f(s) = {
+            var x, y, val : R; 
+            if (witness \notin qs) {
+                (x, y) <- F.query();
+                qs.[witness] <- (x, y);
+            } else {
+                (x, y) <- oget qs.[witness];
+            }
+            if (s) {
+                val <- y;
+            } else {
+                val <- x;
+            }
+            
+            return val;
+        }
+    }    
 
     proc distinguish() = {
-        var b;
-        b <@ A(O).solve();
+        var b : bool;
+        O.init();
+        b <@ D(O).distinguish();
         return b;
     }
 }.
 
-lemma sample_dR_iso g: mu1 sample g = mu1 dR (act g x0).
-proof.
-have /= <- := dmap1E_can DR.dunifin (extract x0) (fun g=> act g x0) g _ _.
-+ by rewrite /cancel=> g'; rewrite -extractUniq.
-+ by move=> a _ /=; rewrite extractP.
-congr; apply: eq_funi_ll.
-+ exact: DG.dunifin_funi.
-+ exact: DG.dunifin_ll.
-+ apply/dmap_funi.
-+ exists (fun g=> act g x0); split.
-  + by move=> a; exact: extractP.
-  by move=> h; rewrite -extractUniq.
-exact: dunifin_funi.
-exact/dmap_ll/dunifin_ll.
-qed.
 
-lemma Hybrid_WPR_WP_Real_eq (A <: Hybrid_WPR_Adv{Hybrid_WPR_Real, WP_Real}) (x : int) &m:
-   Pr[WP_IND(WP_Real, B1(A)).main(x) @ &m: res] = Pr[Hybrid_WPR_IND(Hybrid_WPR_Real, A).main(x) @ &m: res].
+lemma Hybrid_PRF_WPR_Real_eq (D <: Distinguisher{Hybrid_PRF_0', Hybrid_WP_Real, C}) &m :
+    Pr[IND(Hybrid_PRF_0', D).main() @ &m: res] = Pr[WP_IND(Hybrid_WP_Real, C(D)).main() @ &m: res].
 proof.
-byequiv (: ={glob A, arg} ==> ={res})=> //.
-proc; inline *.
-wp.
-call (:    ={c, q}(WP_Real, Hybrid_WPR_Real)
-        /\ WP_Real.g{1} = Hybrid_WPR_Real.gt{2}).
-+ proc; if; auto.
-  rnd (extract x0) (transpose act x0); auto=> /> &2 c_le_q.
-  split=> [g _|_]; first exact: extractUniq.
-  split=> [g _|_ xq _]; first exact: sample_dR_iso.
-  by rewrite extractP.
-by auto.
-qed.
-
-lemma Hybrid_WPR_WP_Ideal_eq (A <: Hybrid_WPR_Adv{Hybrid_WPR_Ideal, WP_Ideal}) (x : int) &m:
-   Pr[WP_IND(WP_Ideal, B1(A)).main(x) @ &m: res] = Pr[Hybrid_WPR_IND(Hybrid_WPR_Ideal, A).main(x) @ &m: res].
-proof.
+(* byequiv (: ={glob D, arg} ==> ={res})=> //.*)
 byequiv=> //.
 proc.
 inline *.
 wp.
+seq 1 1 : (Hybrid_PRF_0'.g1{1} = Hybrid_WP_Real.gt{2}
+            /\ ={glob D}).
++ by rnd.
 sp.
-call (: WP_Ideal.c{1} = Hybrid_WPR_Ideal.c{2}
-     /\ WP_Ideal.q{1} = Hybrid_WPR_Ideal.q{2}
-     ).
-+ proc.
-  if.
-  + by move=> />.
-  + seq 1 2 : (={xq}
-              /\ WP_Ideal.c{1} = Hybrid_WPR_Ideal.c{2}
-              /\ WP_Ideal.q{1} = Hybrid_WPR_Ideal.q{2}
-              ).
-    wp.    
-    rnd (fun x => extract x0 x) (fun g => act g x0).
-    skip=> &1 &2 /> le.
-    split.
-    + move=> g _.
-        exact extractUniq.
-    move=> _.
-    split.
-    + move=> g _.
-        have /= <- := dmap1E_can DR.dunifin (extract x0) (fun g=> act g x0) g _ _.
-        + by rewrite /cancel=> g'; rewrite -extractUniq.
-        + by move=> a _ /=; rewrite extractP.
-        congr; apply: eq_funi_ll.
-        + exact: DG.dunifin_funi.
-        + exact: DG.dunifin_ll.
-        + apply/dmap_funi.
-        + exists (fun g=> act g x0); split.
-            + by move=> a; exact: extractP.
-            by move=> h; rewrite -extractUniq.
-        exact: dunifin_funi.
-        exact/dmap_ll/dunifin_ll.
-    move=> _ r rin.
-    by rewrite extractP.    
-    wp.
-    rnd (fun x => extract xq{1} x) (fun g => act g xq{2}).
-    skip=> &1 &2 />.
-    split.
-    + move=> g _.
-        exact extractUniq.
-    move=> _.
-    split.
-    + move=> g _.
-        have /= <- := dmap1E_can DR.dunifin (extract xq{2}) (fun g=> act g xq{2}) g _ _.
-        + by rewrite /cancel=> g'; rewrite -extractUniq.
-        + by move=> a _ /=; rewrite extractP.
-        congr; apply: eq_funi_ll.
-        + exact: DG.dunifin_funi.
-        + exact: DG.dunifin_ll.
-        + apply/dmap_funi.
-        + exists (fun g=> act g xq{2}); split.
-            + by move=> a; exact: extractP.
-            by move=> h; rewrite -extractUniq.
-        exact: dunifin_funi.
-        exact/dmap_ll/dunifin_ll.
-    move=> _ r rin.
-    by rewrite extractP.   
-  wp.
-  by skip=> />.
-by skip=> />.
+call (:   Hybrid_PRF_0'.g1{1} = Hybrid_WP_Real.gt{2}
+       /\ (0 \notin Hybrid_PRF_0'.m{1} <=> witness \notin C.O.qs{2})
+       /\ act (oget Hybrid_PRF_0'.m.[0]{1}) x0 = (oget C.O.qs.[witness]).`1{2}
+       /\ act Hybrid_PRF_0'.g1{1} (act (oget Hybrid_PRF_0'.m.[0]{1}) x0) = (oget C.O.qs.[witness]).`2{2}).
++ proc; sp; inline*.
+  sp.
+  if=> />.
+  + auto=> &1 &2 /> _ _ _ g h.
+    rewrite !mem_set.
+    auto=> _ />.
+    by rewrite !get_set_sameE !Core.oget_some.
+  by auto=> &1 &2 />.
+auto=> &1 &2 />.
+rewrite !emptyE !Core.oget_none.
+do split; first 2 by apply contra; rewrite !emptyE.
+(* Seems reasonable but also not, can a witness act? can you take the fst*)
+admit.
+admit.
 qed.
 
-lemma Hybrid_WPR_WP_eq (A <: Hybrid_WPR_Adv{Hybrid_WPR_Ideal, Hybrid_WPR_Real, WP_Real, WP_Ideal}) (x : int) &m : 
-`|Pr[Hybrid_WPR_IND(Hybrid_WPR_Real, A).main(x) @ &m: res] - Pr[Hybrid_WPR_IND(Hybrid_WPR_Ideal, A).main(x) @ &m: res]| 
-= `| Pr[WP_IND(WP_Real, B1(A)).main(x) @ &m: res] - Pr[WP_IND(WP_Ideal, B1(A)).main(x) @ &m: res] |.
-by rewrite (Hybrid_WPR_WP_Real_eq A) (Hybrid_WPR_WP_Ideal_eq A).
+lemma Hybrid_PRF_WPR_Ideal_eq (D <: Distinguisher{Hybrid_PRF_L, Hybrid_WP_Ideal, C}) &m :
+    Pr[IND(Hybrid_PRF_L, D).main() @ &m: res] = Pr[WP_IND(Hybrid_WP_Ideal, C(D)).main() @ &m: res].
+proof.
+byequiv (: ={glob D, arg} ==> ={res})=> //.
+proc.
+inline *.
+sp.
+wp.
+admit.
 qed.
